revert Pipeline.v to PipelineWithRename.v from master

compiler/src/compiler/Pipeline.v
@@ -2,6 +2,7 @@ Require Export Coq.Lists.List.
 Require Import Coq.ZArith.ZArith.
 Export ListNotations.
 Require Export coqutil.Decidable.
+Require Import coqutil.Tactics.ParamRecords.
 Require        compiler.ExprImp.
 Require Export compiler.FlattenExprDef.
 Require Export compiler.FlattenExpr.
@@ -32,7 +33,6 @@ Require Export riscv.Utility.InstructionCoercions.
 Require Import compiler.SeparationLogic.
 Require Import coqutil.Tactics.Simp.
 Require Import compiler.FlattenExprSimulation.
-Require Import compiler.Spilling.
 Require Import compiler.RegRename.
 Require Import compiler.FlatToRiscvSimulation.
 Require Import compiler.Simulation.
@@ -117,117 +117,6 @@ Module Import Pipeline.
 
 End Pipeline.
 
-Section SIM.
-  Context {Frame1 State1: Type}.
-  Context (exec1: State1 -> (State1 -> Prop) -> Prop).
-  Context {Frame2 State2: Type}.
-  Context (exec2: State2 -> (State2 -> Prop) -> Prop).
-  Context (states_related: Frame1 -> Frame2 -> State1 -> State2 -> Prop).
-
-  Definition simulation f1 f2 :=
-      forall (P1: State1 -> Prop) (P2: State2 -> Prop),
-      (* read line below as "P2 must be implied by exists s1', states_related f1 f2 s1' s2' /\ P1 s1'"
-         or as "if P1 says s1' is an acceptable final state, then P2 must accept all s2' related to s1'" *)
-      (forall s1' s2', states_related f1 f2 s1' s2' -> P1 s1' -> P2 s2') ->
-      forall s1 s2, states_related f1 f2 s1 s2 -> exec1 s1 P1 -> exec2 s2 P2.
-
-  (* Note: The above could be simplified like this, but then P2 cannot be weakened and we need
-     to carry around a separate hypothesis requiring weakening for language 2. *)
-  Definition simulation_without_weakening f1 f2 := forall (P1: State1 -> Prop) s1 s2,
-      states_related f1 f2 s1 s2 ->
-      exec1 s1 P1 ->
-      exec2 s2 (fun s2' => exists s1', states_related f1 f2 s1' s2' /\ P1 s1').
-
-  Lemma simulation_alt: forall f1 f2, simulation f1 f2 -> simulation_without_weakening f1 f2.
-  Proof. unfold simulation, simulation_without_weakening. eauto 10. Qed.
-
-  Lemma simulation_alt_verboseproof: forall f1 f2, simulation f1 f2 -> simulation_without_weakening f1 f2.
-  Proof.
-    unfold simulation, simulation_without_weakening.
-    intros *. intro Sim. intros. eapply Sim. 2,3: eassumption.
-    clear. intros. eauto.
-  Qed.
-
-  Lemma simulation_alt':
-    (forall (P2 P2': State2 -> Prop), (forall s2, P2 s2 -> P2' s2) -> forall s2, exec2 s2 P2 -> exec2 s2 P2') ->
-    forall f1 f2, simulation_without_weakening f1 f2 -> simulation f1 f2.
-  Proof.
-    unfold simulation_without_weakening, simulation.
-    intros W. intros *. intros Sim. intros.
-    eapply W. 2: {
-      eapply Sim. 1: eassumption. eassumption.
-    }
-    cbv beta.
-    intros s (s1' & ? & ?).
-    eauto.
-  Qed.
-
-End SIM.
-
-Section COMPOSE.
-  Context {Frame1 State1: Type}.
-  Context (exec1: State1 -> (State1 -> Prop) -> Prop).
-  Context {Frame2 State2: Type}.
-  Context (exec2: State2 -> (State2 -> Prop) -> Prop).
-  Context {Frame3 State3: Type}.
-  Context (exec3: State3 -> (State3 -> Prop) -> Prop).
-  Context (frelated12: Frame1 -> Frame2 -> Prop).
-  Context (frelated23: Frame2 -> Frame3 -> Prop).
-  Context (related12: Frame1 -> Frame2 -> State1 -> State2 -> Prop).
-  Context (related23: Frame2 -> Frame3 -> State2 -> State3 -> Prop).
-
-(*
-  Definition compose_frelated: Frame1 -> Frame3 -> Prop :=
-    fun f1 f3 => exists f2, frelated12 f1 f2 /\ frelated23 f2 f3.
-*)
-
-  Definition compose_related(f2: Frame2)(f1: Frame1)(f3: Frame3): State1 -> State3 -> Prop :=
-    fun s1 s3 => exists s2, related12 f1 f2 s1 s2 /\ related23 f2 f3 s2 s3.
-
-  Lemma compose_simulation
-        (S12: forall f1 f2, frelated12 f1 f2 -> simulation exec1 exec2 related12 f1 f2)
-        (S23: forall f2 f3, frelated23 f2 f3 -> simulation exec2 exec3 related23 f2 f3):
-    forall f1 f3 f2, frelated12 f1 f2 -> frelated23 f2 f3 ->
-    simulation exec1 exec3 (compose_related f2) f1 f3.
-  Proof.
-  Abort.
-(* how to say that middle frame is still the same in post? above can, but makes simulation uncomposable
-   previous approach didn't achieve that
-
-
-each simulation holds under some assumptions about frames, and assuming intermediate frames exist
-compose two simulations that live under assumptions, combining the list of assumptions?
-
-
-forall (a1: A1) ... (an: An), A
-forall (b1: B1) ... (bm: Bm), B
-
-forall (a1: A1) ... (an: An)(b1: B1) ... (bm: Bm), compose A B
-
-forall (a: {A1 * ... An | P}), A
-
-real parameterization only needed in last phase
-
-but previous phases might have target-language-state validity (and thus "related") depend on source program
-
-
-
-    unfold simulation, compose_frelated, compose_related in *.
-    intros f1 f3 (f2 & HF12 & HF23) P1 P3 P13 s1 s3 (f2 & s2 & HR12 & HR23) Ex1.
-    eapply S23. 2: exact HR23. 2: {
-      eapply S12 with (P2 := (fun s2' => exists s1', related12 f1 s1' f2 s2' /\ P1 s1')).
-      2: exact HR12. 2: exact Ex1. eauto. }
-    intros s2' s3' HR23' (s1' & HR12' & p1). eauto.
-  Qed.
-
-*)
-
-(* simulation  nil/cons ? *)
-
-End COMPOSE.
-
-Arguments compose_simulation {_} {_} {_} {_} {_} {_} {_} {_} {_} {_} {_}.
-
 Section Pipeline1.
 
   Context {p: parameters}.
@@ -261,21 +150,22 @@ Section Pipeline1.
   Local Notation flat_env := (@string_keyed_map p (list string * list string * FlatImp.stmt string)).
   Local Notation renamed_env := (@string_keyed_map p (list Z * list Z * FlatImp.stmt Z)).
 
-  Definition flattenPhase(prog: source_env): option flat_env := flatten_functions prog.
+  Definition flattenPhase(prog: source_env): option flat_env := flatten_functions (2^10) prog.
   Definition renamePhase(prog: flat_env): option renamed_env :=
     rename_functions prog.
-  Definition spillingPhase(prog: renamed_env): option renamed_env := Some (spill_functions prog).
 
   (* Note: we could also track code size from the source program all the way to the target
      program, and a lot of infrastructure is already there, will do once/if we want to get
      a total compiler.
      Returns the fun_pos_env so that users know where to jump to call the compiled functions. *)
-  Definition riscvPhase(prog: renamed_env):
-    option (list Instruction * funname_env Z * Z) :=
-    bind_opt stack_words_needed <- stack_usage prog;
+  Definition riscvPhase(ml: MemoryLayout)(prog: renamed_env):
+    option (list Instruction * funname_env Z) :=
+    bind_opt stack_needed <- stack_usage prog;
+    let num_stackwords := word.unsigned (word.sub ml.(stack_pastend) ml.(stack_start)) / bytes_per_word in
+    if Z.ltb num_stackwords stack_needed then None (* not enough stack *) else
     let positions := FlatToRiscvDef.build_fun_pos_env prog in
     let '(i, _) := FlatToRiscvDef.compile_funs positions prog in
-    Some (i, positions, stack_words_needed).
+    Some (i, positions).
 
   Definition composePhases{A B C: Type}(phase1: A -> option B)(phase2: B -> option C)(a: A) :=
     match phase1 a with
@@ -283,235 +173,51 @@ Section Pipeline1.
     | None => None
     end.
 
-  Definition composed_compile: source_env -> option (list Instruction * funname_env Z * Z) :=
+  Definition compile(ml: MemoryLayout):
+    source_env -> option (list Instruction * funname_env Z) :=
     (composePhases flattenPhase
     (composePhases renamePhase
-    (composePhases spillingPhase
-                   riscvPhase))).
+                   (riscvPhase ml))).
 
-  Definition FlatState(varname: Type){pp : FlatImp.parameters varname}: Type :=
-    FlatImp.env * FlatImp.stmt varname * bool * FlatImp.trace * FlatImp.mem * FlatImp.locals * MetricLog.
+  Section Sim.
+    Context (ml: MemoryLayout)
+            (mlOk: MemoryLayoutOk ml)
+            (f_entry_rel_pos : Z)
+            (f_entry_name : string)
+            (p_call: word) (* address where the call to the entry function is stored *)
+            (p_functions: word) (* address where the compiled functions are stored *)
+            (Rdata Rexec : FlatToRiscvCommon.mem -> Prop)
+            (prog: renamed_env)
+            (e1 : FlattenExpr.ExprImp_env)
+            (e2 : FlattenExpr.FlatImp_env)
+            (funname : string)
+            (Hf: flatten_functions (2 ^ 10) e1 = Some e2).
+    Let c2 := (@FlatImp.SSeq String.string FlatImp.SSkip (FlatImp.SCall [] funname [])).
+    Let c3 := (@FlatImp.SSeq Z FlatImp.SSkip (FlatImp.SCall [] f_entry_name [])).
+    Context (av' : Z) (r' : string_keyed_map Z)
+            (ER: envs_related e2 prog)
+            (Ren: rename map.empty c2 lowest_available_impvar = Some (r', c3, av'))
+            (H_p_call: word.unsigned p_call mod 4 = 0)
+            (H_p_functions: word.unsigned p_functions mod 4 = 0)
+            (G: map.get (FlatToRiscvDef.build_fun_pos_env prog) f_entry_name = Some f_entry_rel_pos)
+            (F: fits_stack 0 (word.unsigned (word.sub (stack_pastend ml) (stack_start ml)) / bytes_per_word) prog
+                           (FlatImp.SSeq FlatImp.SSkip (FlatImp.SCall [] f_entry_name [])))
+            (GEI: good_e_impl prog (FlatToRiscvDef.build_fun_pos_env prog)).
 
-  Definition flatExec{varname: Type}{pp : FlatImp.parameters varname}:
-    FlatState varname -> (FlatState varname -> Prop) -> Prop :=
-    fun '(e, s, done, t, m, l, mc) post =>
-      done = false /\
-      FlatImp.exec e s t m l mc (fun t' m' l' mc' => post (e, s, true, t', m', l', mc')).
+    Definition flattenSim: simulation _ _ _ :=
+      FlattenExprSimulation.flattenExprSim (2^10) e1 e2 funname Hf.
+    Definition regAllocSim: simulation _ _ _ :=
+      renameSim (@ext_spec p)
+                e2 prog c2 c3 av' r' ER Ren.
+    Definition flatToRiscvSim: simulation _ _ _ :=
+      FlatToRiscvSimulation.flatToRiscvSim
+        f_entry_rel_pos f_entry_name p_call Rdata Rexec
+        p_functions ml.(stack_start) ml.(stack_pastend)
+        prog compile_ext_call_correct H_p_call H_p_functions G F GEI.
 
-  (* Note: contrary to GhostConsts, this record only contains risc-v-related types, no FlatImp-related types *)
-  Record RiscvFrame: Type := {
-    addr_functions: word;
-    insts_functions: list Instruction;
-    addr_snippet: word;
-    insts_snippet: list Instruction;
-    stack_start: word;
-    stack_pastend: word;
-    xframe: mem -> Prop;
-    dframe: mem -> Prop;
-  }.
-
-  Definition satisfiesRiscvFrame(done: bool)(f: RiscvFrame)(mach: MetricRiscvMachine): Prop :=
-      (program iset f.(addr_functions) f.(insts_functions) *
-       program iset f.(addr_snippet) f.(insts_snippet) *
-       mem_available f.(stack_start) f.(stack_pastend) *
-       f.(dframe) * f.(xframe)
-      )%sep mach.(getMem) /\
-      subset (footpr (program iset f.(addr_functions) f.(insts_functions) *
-                      program iset f.(addr_snippet) f.(insts_snippet) *
-                      f.(xframe))%sep)
-             (of_list (getXAddrs mach)) /\
-      word.unsigned (mach.(getPc)) mod 4 = 0 /\
-      mach.(getPc) = (if done
-                      then word.add f.(addr_snippet) (word.of_Z (4 * Z.of_nat (length f.(insts_snippet))))
-                      else f.(addr_snippet)) /\
-      mach.(getNextPc) = word.add mach.(getPc) (word.of_Z 4) /\
-      regs_initialized mach.(getRegs) /\
-      map.get mach.(getRegs) RegisterNames.sp = Some f.(stack_pastend) /\
-      (* configured by PrimitivesParams, can contain invariants needed for external calls *)
-      valid_machine mach.
-
-  Definition flat_related_to_riscv
-             (frame1: @FlatImp.env Z _ * FlatImp.stmt Z)(s1: FlatState Z)
-             (frame2: RiscvFrame)(s2: MetricRiscvMachine): Prop :=
-    let '(e, c, done, t, m, l, mc) := s1 in
-    frame1 = (e, c) /\
-    map.extends s2.(getRegs) l /\
-    s2.(getLog) = t /\
-    fits_stack 0 (word.unsigned (word.sub frame2.(stack_pastend) frame2.(stack_start))) e c /\
-    FlatToRiscvDef.stmt_not_too_big c /\
-    FlatToRiscvDef.valid_FlatImp_vars c /\
-    let relpos := (word.unsigned (word.sub frame2.(addr_snippet) frame2.(addr_functions))) in
-    let e_pos := FlatToRiscvDef.build_fun_pos_env e in
-    fst (FlatToRiscvDef.compile_funs e_pos e) = frame2.(insts_functions) /\
-    FlatToRiscvDef.compile_stmt e_pos relpos 0 c = frame2.(insts_snippet) /\
-    satisfiesRiscvFrame done frame2 s2 /\
-    good_e_impl e e_pos.
-
-  Axiom TODO: False.
-
-(*
-  Lemma flatToRiscvSim: simulation flatExec FlatToRiscvCommon.runsTo flat_related_to_riscv.
-  Proof.
-    unfold simulation, flatExec, FlatState, FlatImp.SimExec, flat_related_to_riscv.
-    intros.
-    destruct s1 as ((((((e & c) & done) & t) & m) & l) & mc).
-    destruct_RiscvMachine s2.
-    simp.
-    eapply runsTo_weaken.
-    - specialize compile_stmt_correct with (1 := @compile_ext_call_correct _ h).
-      unfold compiles_FlatToRiscv_correctly. intros compile_stmt_correct.
-      eapply compile_stmt_correct.  all: case TODO. with (g := f2); clear compile_stmt_correct; simpl.
-      + eassumption.
-      + clear. intros k v ?. eassumption.
-      + assumption.
-      + eauto using fits_stack_call.
-      + eassumption.
-      + eassumption.
-      + eassumption.
-      + assert (word.ok word) by exact Utility.word_ok.
-        solve_divisibleBy4.
-        case TODO.
-      + assert (word.ok word) by exact Utility.word_ok.
-        solve_divisibleBy4.
-        case TODO.
-      + (* TODO why are these manual steps needed? *)
-        case TODO.
-      + assert (word.ok word) by exact Utility.word_ok.
-        case TODO.
-      + assumption.
-    - simpl. intros. simp.
-      eapply H. 2: eassumption.
-      cbv beta iota.
-      repeat match goal with
-             | |- _ /\ _ => split
-             | _ => eassumption
-             | _ => reflexivity
-             end.
-
-      Unshelve. all: case TODO.
-    - case TODO.
-  Qed.
-*)
-
-  Definition spilling_related
-             (frame1: @FlatImp.env Z _ * FlatImp.stmt Z)(s1: FlatState Z)
-             (frame2: @FlatImp.env Z _ * FlatImp.stmt Z)(s2: FlatState Z) :=
-    let '(e1, c1, done1, t1, m1, l1, mc1) := s1 in
-    let '(e2, c2, done2, t2, m2, l2, mc2) := s2 in
-    frame1 = (e1, c1) /\
-    frame2 = (e2, c2) /\
-    done1 = done2 /\
-    c2 = spill_stmt c1 /\
-    exists maxvar (fpval: word),
-      Spilling.envs_related e1 e2 /\
-      Spilling.valid_vars_src maxvar c1 /\
-      Spilling.related ext_spec maxvar (emp True) fpval t1 m1 l1 t2 m2 l2.
-
-  Lemma spilling_sim: simulation flatExec flatExec spilling_related.
-  Proof.
-    unfold simulation, flatExec, spilling_related. intros f1 f2 P1 P2 R.
-    intros ((((((e1 & c1) & done1) & t1) & m1) & l1) & mc1) ((((((e2 & c2) & done2) & t2) & m2) & l2) & mc2).
-    intros. simp. split; [reflexivity|].
-    eapply FlatImp.exec.weaken.
-    - eapply spilling_correct; eassumption.
-    - cbv beta. intros. simp. eapply R. 2: eassumption. simpl.
-      eauto 10.
-  Qed.
-
-  Definition renaming_related
-             (frame1: @FlatImp.env string _ * FlatImp.stmt string)(s1: FlatState string)
-             (frame2: @FlatImp.env Z _ * FlatImp.stmt Z)(s2: FlatState Z) :=
-    let '(e1, c1, done1, t1, m1, l1, mc1) := s1 in
-    let '(e2, c2, done2, t2, m2, l2, mc2) := s2 in
-    frame1 = (e1, c1) /\
-    frame2 = (e2, c2) /\
-    done1 = done2 /\
-    RegRename.envs_related e1 e2 /\
-    (exists r' av', RegRename.rename map.empty c1 lowest_available_impvar = Some (r', c2, av')) /\
-    t1 = t2 /\
-    m1 = m2 /\
-    (done1 = false -> l1 = map.empty /\ l2 = map.empty /\ mc1 = mc2).
-
-  Lemma renaming_sim: simulation flatExec flatExec renaming_related.
-  Proof.
-    unfold simulation, flatExec, renaming_related. intros f1 f2 P1 P2 R.
-    intros ((((((e1 & c1) & done1) & t1) & m1) & l1) & mc1) ((((((e2 & c2) & done2) & t2) & m2) & l2) & mc2).
-    intros. simp. split; [reflexivity|]. specialize (Hp3 eq_refl). simp.
-    pose proof Hp1 as A.
-    apply rename_props in A;
-      [|eapply map.empty_injective|eapply dom_bound_empty].
-    simp.
-    eapply FlatImp.exec.weaken.
-    - eapply rename_correct.
-      1: eassumption.
-      1: eassumption.
-      3: {
-        eapply Ap2. eapply TestLemmas.extends_refl.
-      }
-      1: eassumption.
-      1: eassumption.
-      unfold states_compat. intros *. intro B.
-      erewrite map.get_empty in B. discriminate.
-    - simpl. intros. simp.
-      eapply R. 2: eassumption. simpl. clear R. intuition (discriminate || eauto).
-  Qed.
-
-  Definition SrcState: Type :=
-    Semantics.env * Syntax.cmd * bool * Semantics.trace * Semantics.mem * Semantics.locals * MetricLog.
-
-  Definition srcExec: SrcState -> (SrcState -> Prop) -> Prop :=
-    fun '(e, c, done, t, m, l, mc) post =>
-      done = false /\
-      Semantics.exec e c t m l mc (fun t' m' l' mc' => post (e, c, true, t', m', l', mc')).
-
-  Definition flattening_related
-             (frame1: Semantics.env * Syntax.cmd)(s1: SrcState)
-             (frame2: @FlatImp.env string _ * FlatImp.stmt string)(s2: FlatState string) :=
-    let '(e1, c1, done1, t1, m1, l1, mc1) := s1 in
-    let '(e2, c2, done2, t2, m2, l2, mc2) := s2 in
-    frame1 = (e1, c1) /\
-    frame2 = (e2, c2) /\
-    done1 = done2 /\
-    ExprImp2FlatImp c1 = c2 /\
-    flatten_functions e1 = Some e2 /\
-    t1 = t2 /\
-    m1 = m2 /\
-    (done1 = false -> l1 = map.empty /\ l2 = map.empty /\ mc1 = mc2).
-
-  Lemma flattening_sim: simulation srcExec flatExec flattening_related.
-  Proof.
-    unfold simulation, srcExec, flatExec, flattening_related, ExprImp2FlatImp. intros f1 f2 P1 P2 R.
-    intros ((((((e1 & c1) & done1) & t1) & m1) & l1) & mc1) ((((((e2 & c2) & done2) & t2) & m2) & l2) & mc2).
-    intros. simp. split; [reflexivity|]. specialize (Hp2 eq_refl). simp.
-    eapply FlatImp.exec.weaken.
-    - eapply @flattenStmt_correct_aux with (eH := e1).
-      + typeclasses eauto.
-      + eassumption.
-      + eassumption.
-      + reflexivity.
-      + match goal with
-        | |- ?p = _ => rewrite (surjective_pairing p)
-        end.
-        reflexivity.
-      + intros x k A. rewrite map.get_empty in A. discriminate.
-      + unfold map.undef_on, map.agree_on. intros. reflexivity.
-      + eapply freshNameGenState_disjoint.
-    - simpl. intros. simp. eapply R. 2: eassumption. simpl. intuition (discriminate || eauto).
-  Qed.
-
-  Definition related: Semantics.env * Syntax.cmd -> SrcState -> RiscvFrame -> MetricRiscvMachine -> Prop :=
-    (compose_related flattening_related
-    (compose_related renaming_related
-    (compose_related spilling_related
-                     flat_related_to_riscv))).
-
-  Lemma sim: simulation srcExec FlatToRiscvCommon.runsTo related.
-  Proof.
-    exact (compose_simulation flattening_sim
-          (compose_simulation renaming_sim
-          (compose_simulation spilling_sim
-                              flatToRiscvSim))).
-  Qed.
+    Definition sim: simulation _ _ _ :=
+      (compose_sim flattenSim (compose_sim regAllocSim flatToRiscvSim)).
+  End Sim.
 
   Lemma rename_fun_valid: forall argnames retnames body impl',
       rename_fun (argnames, retnames, body) = Some impl' ->
@@ -536,8 +242,6 @@ Section Pipeline1.
     { assumption. }
     { assumption. }
     simp.
-    set (lowest_nonregister := 32).
-    assert (Z.leb z1 lowest_nonregister = true) as E2 by case TODO.
     ssplit.
     - eapply Forall_impl. 2: {
         eapply map.getmany_of_list_in_map. eassumption.
@@ -622,9 +326,9 @@ Section Pipeline1.
 
   Local Definition FlatImp__word_eq : FlatImp.word -> FlatImp.word -> bool := word.eqb.
   Local Instance  EqDecider_FlatImp__word_eq : EqDecider FlatImp__word_eq.
-  Proof. eapply word.eqb_spec. Unshelve. exact word_ok. Qed.
+  Proof. eapply word.eqb_spec. Unshelve. all: exact word_ok. Qed.
 
-  Lemma mem_available_to_exists: forall start pastend m P,
+  Lemma mem_available_to_exists: forall start pastend (m: mem) P,
       (mem_available start pastend * P)%sep m ->
       exists anybytes,
         Z.of_nat (List.length anybytes) = word.unsigned (word.sub pastend start) /\
@@ -637,7 +341,7 @@ Section Pipeline1.
     eauto.
   Qed.
 
-  Definition mem_to_available: forall start pastend m P anybytes,
+  Definition mem_to_available: forall start pastend (m: mem) P anybytes,
      Z.of_nat (List.length anybytes) = word.unsigned (word.sub pastend start) ->
      (ptsto_bytes start anybytes * P)%sep m ->
      (mem_available start pastend * P)%sep m.
@@ -678,7 +382,7 @@ Section Pipeline1.
   Qed.
 
   Lemma stack_length_divisible: forall (ml: MemoryLayout) {mlOk: MemoryLayoutOk ml},
-    word.unsigned (word.sub (MemoryLayout.stack_pastend ml) (MemoryLayout.stack_start ml)) mod bytes_per_word = 0.
+    word.unsigned (word.sub (stack_pastend ml) (stack_start ml)) mod bytes_per_word = 0.
   Proof.
     intros.
     destruct mlOk.
@@ -800,14 +504,12 @@ Section Pipeline1.
      is layed out in memory), while 2) should be commutative because the "function"
      separation logic predicate it seps onto the separation logic formula is the same
      if we pass it the same function position map. *)
-  Lemma functions_to_program: forall functions_start e instrs pos_map stack_size,
-      riscvPhase e = Some (instrs, pos_map, stack_size) ->
+  Lemma functions_to_program: forall ml functions_start e instrs pos_map,
+      riscvPhase ml e = Some (instrs, pos_map) ->
       iff1 (program iset functions_start instrs)
            (FlatToRiscvCommon.functions functions_start (FlatToRiscvDef.build_fun_pos_env e) e).
   Proof.
-    (* PARAMRECORDS *)
-    assert (map.ok FlatImp.env). { unfold FlatImp.env. simpl. typeclasses eauto. }
-    assert (map.ok mem) as Ok by exact mem_ok.
+    assert nat as H by exact O. (* preserve names *)
 
     unfold riscvPhase.
     intros.
@@ -823,13 +525,13 @@ Section Pipeline1.
       destruct H0. apply H1; clear H1.
       intros. rewrite <- H1. f_equal.
       subst.
-      apply (f_equal snd) in E0. simpl in E0. rewrite <- E0.
+      apply (f_equal snd) in E1. simpl in E1. rewrite <- E1.
       transitivity (snd (map.fold (FlatToRiscvDef.add_compiled_function map.empty) ([], map.empty) e)).
       - unfold FlatToRiscvDef.build_fun_pos_env, snd. reflexivity.
       - apply build_fun_pos_env_ignores_posmap.
     }
-    revert E0.
-    revert instrs r. clear E stack_size.
+    revert E1.
+    revert instrs r. clear E E0 z.
     eapply (map.fold_spec (R:=(list Instruction * _))) with (m:=e); repeat (cbn || simp || intros).
     { rewrite map.fold_empty. intuition try reflexivity.
       - eapply H0. eapply map.get_empty.
@@ -843,8 +545,8 @@ Section Pipeline1.
       cancel. }
     case r as (instrs'&r').
     specialize H1 with (1 := eq_refl).
-    unfold FlatToRiscvDef.add_compiled_function in E0.
-    injection E0; clear E0; intros. subst.
+    unfold FlatToRiscvDef.add_compiled_function in E1.
+    injection E1; clear E1; intros. subst.
     unfold program in *.
     wseplog_pre.
     destruct H1.
@@ -900,246 +602,6 @@ Section Pipeline1.
       (* configured by PrimitivesParams, can contain invariants needed for external calls *)
       valid_machine mach.
 
-  (* handwritten "related" (rather than composition of all phases), and restricted to
-     argument-less function calls (compiling general snippets need more context for
-     FlatToRiscv, namely function positions) and thus simpler *)
-  Definition manual_related(f1: Semantics.env * Syntax.cmd.cmd)(s1: SrcState)
-                           (f2: GhostConsts)(mach: MetricRiscvMachine): Prop :=
-    let '(functions, c) := f1 in
-    let '(functions', c', done, t, mH, lH, mcH) := s1 in
-    functions' = functions /\
-    c' = c /\
-    mach.(getLog) = t /\
-    (done = false -> lH = map.empty) /\
-    exists f_entry_name f_entry_rel_pos (finstrs: list Instruction) stack_start stack_words_needed,
-      c = Syntax.cmd.call [] f_entry_name [] /\
-      ExprImp.valid_funs functions /\
-      composed_compile functions = Some (finstrs, f2.(e_pos), stack_words_needed) /\
-      map.get f2.(e_pos) f_entry_name = Some f_entry_rel_pos /\
-      machine_ok f2.(program_base) f_entry_rel_pos
-                 stack_start f2.(p_sp) finstrs
-                 f2.(p_insts) (if done then (word.add f2.(p_insts) (word.of_Z 4)) else f2.(p_insts))
-                 mH f2.(FlatToRisc... ? dframe) f2.(xframe) mach /\
-      f2.(rem_stackwords) = word.unsigned (word.sub f2.(p_sp) stack_start) /\
-      f2.(rem_framewords) = 0 /\
-      stack_words_needed <= f2.(rem_stackwords) / bytes_per_word /\
-      f2.(insts) = [[Jal RegisterNames.ra
-                         (f_entry_rel_pos + word.signed (word.sub f2.(program_base) f2.(p_insts)))]].
-
-manual_related new?
-
-  Ltac sim'_destructible T :=
-    lazymatch T with
-    | prod _ _ => idtac
-    | SrcState => idtac
-    | FlatState _ => idtac
-    | GhostConsts => idtac
-    end.
-
-  Lemma rename_functions_related: forall e1 e2,
-    rename_functions e1 = Some e2 ->
-    RegRename.envs_related e1 e2.
-  Proof.
-    intros.
-    unfold envs_related.
-    intros f [ [argnames resnames] body1 ] G.
-    unfold rename_functions in *.
-    eapply map.map_all_values_fw.
-    5: exact G. 4: eassumption.
-    - eapply String.eqb_spec.
-    - typeclasses eauto.
-    - typeclasses eauto.
-  Qed.
-
-  Create HintDb simpl_related.
-  Hint Resolve rename_functions_related : simpl_related.
-
-
-  (* Some compilation phases establish some kind of "validFrame" for the target language,
-     eg spilling guarantees that all register names are <32 *, and these "validFrame"
-     conditions are then needed by the next phase's "related".
-     (making "validFrame" a distinct concept might be overkill, and not work so well for
-     risc-v because it would need the high-level memory as well to split the memory).
-     Filling in the intermediate existentials created by compose_related and showing that
-     the compilation of phase i respects the "validFrame" conditions of phase i+1 is the
-     purpose of this proof. *)
-
-  (* where to go from "compile hl = ll" to "envs_related hl ll"?
-     ideally in each phase simulation, rather than after the composition *)
-
-  Lemma sim': simulation srcExec runsTo manual_related.
-  Proof.
-    eapply specialize_simulation_frames. 3: eapply sim.
-    - unfold related, compose_related.
-      unfold flattening_related, renaming_related, spilling_related, flat_related_to_riscv.
-      unfold manual_related, machine_ok, goodMachine.
-      unfold composed_compile, composePhases.
-      unfold flattenPhase, renamePhase, spillingPhase, riscvPhase.
-
-Ltac step := match goal with
-             | x: ?T |- _ => sim'_destructible T; destruct x
-             | |- forall _, _ => intros
-             | |- _ => progress (cbn in *; simp)
-             | |- exists x: ?T, _ =>
-               let y := fresh x in unshelve epose (_: T) as y;
-               [ repeat lazymatch goal with
-                        | |- ?T => sim'_destructible T; econstructor
-                        end;
-                 shelve
-               | exists y; subst y ]
-             | |- _ /\ _ => split
-           (*| |- ?G => assert_fails (has_evar G); reflexivity*)
-             | |- ?G => reflexivity
-             | |- _ => eauto 3 with simpl_related
-             end.
-
-      repeat step.
-
-
-      {
-
-Search r3.
-
-(* problem with GhostConsts: contains e_impl, which is a concept from FlatImp, can't easily
-   be derived by looking at RiscvMachine state (would need to decompile) *)
-
-  E2 : FlatToRiscvDef.compile_funs (FlatToRiscvDef.build_fun_pos_env (spill_functions r3))
-         (spill_functions r3) = (finstrs, r4)
-
-spill_functions r3 = e_impl   ?
-
-
-Set Ltac Profiling.
-
-Set Nested Lemmas.
-
-
-E0: rename_functions r1 = Some r3
-
-
-      Search r1.
-
-Show Ltac Profile.
-
-total time:     32.688s
-
- tactic                                   local  total   calls       max
-────────────────────────────────────────┴──────┴──────┴───────┴─────────┘
-─step ----------------------------------  99.8% 100.0%     326   11.103s
-─simp ----------------------------------   0.0%  96.8%     228   11.085s
-─simp_step -----------------------------   0.1%  96.7%     153    0.577s
-─destruct_unique_match -----------------  71.2%  71.2%    2271    0.383s
-─destruct e eqn:N ----------------------  37.6%  37.6%     620    0.057s
-─unique_inversion ----------------------  25.4%  25.4%    4647    0.253s
-─protect_equalities --------------------   8.1%  16.8%    4333    0.015s
-─congruence ----------------------------  13.2%  13.2%    1508    0.018s
-─change_no_check (protected (a = b)) in    8.7%   8.7%   19512    0.011s
-─elimtype ------------------------------   7.3%   7.3%    3021    0.014s
-─discriminate --------------------------   5.7%   5.7%    1513    0.015s
-─destruct e ----------------------------   4.8%   4.8%     137    0.036s
-
- tactic                                   local  total   calls       max
-────────────────────────────────────────┴──────┴──────┴───────┴─────────┘
-─step ----------------------------------  99.8% 100.0%     326   11.103s
-└simp ----------------------------------   0.0%  96.8%     228   11.085s
-└simp_step -----------------------------   0.1%  96.7%     153    0.577s
- ├─destruct_unique_match ---------------  71.2%  71.2%    2271    0.383s
- │ ├─destruct e eqn:N ------------------  37.6%  37.6%     620    0.057s
- │ ├─congruence ------------------------  13.2%  13.2%    1508    0.018s
- │ ├─elimtype --------------------------   7.3%   7.3%    3021    0.014s
- │ ├─discriminate ----------------------   5.7%   5.7%    1513    0.015s
- │ └─destruct e ------------------------   4.8%   4.8%     137    0.036s
- └─unique_inversion --------------------  25.4%  25.4%    4647    0.253s
-  └protect_equalities ------------------   8.1%  16.8%    4333    0.015s
-  └change_no_check (protected (a = b)) i   8.7%   8.7%   19512    0.011s
-
-      Search r.
-
-      step.
-      step.
-      step.
-      step.
-      step.
-      step.
-      step.
-      step.
-      step.
-      step.
-      step.
-      step.
-
-
-step.
-      step.
-      step.
-      step.
-      step.
-      step.
-      step.
-
-      repeat match goal with
-             | x: ?T |- _ => sim'_destructible T; destruct x
-             | |- _ => progress (cbn in *; simp)
-             | |- exists x: ?T, _ =>
-               let y := fresh x in unshelve epose (_: T) as y;
-               [ repeat lazymatch goal with
-                        | |- ?T => sim'_destructible T; econstructor
-                        end;
-                 shelve | ]
-             end.
-      match goal with
-      | |- exists x: ?T, _ =>
-        sim'_destructible T;
-        let y := fresh x in unshelve epose (_: T) as y
-      end.
-      { econstructor; shelve. }
-      exists f2. subst f2.
-      cbn.
-      match goal with
-      | |- exists x: ?T, _ =>
-        let y := fresh x in unshelve epose (_: T) as y
-      end.
-      { repeat lazymatch goal with
-               | |- ?T => sim'_destructible T; econstructor
-               end;
-          shelve. }
-      exists s0.
-      subst s0.
-      cbn.
-
- econstructor.
-
-      match goal with
-      | |- exists x: ?T, _ =>
-        sim'_destructible T;
-        let y := fresh x in evar (y: T)
-      end.
-      exists f2.
-      destruct f2 eqn: E.
-
-      cbn.
-
-      destruct f2.
-      ma
-      intros (e & c).
-      intros ((? & ?) & ?).
-
-
- (e' & c
-      intros. simp.
-
-
-case TODO.
-    - case TODO.
-  Qed.
-
-  Definition compile(ml: MemoryLayout)(p: source_env): option (list Instruction * funname_env Z) :=
-    match composed_compile p with
-    | Some (insts, positions, stack_words_needed) =>
-      let num_stackwords := word.unsigned (word.sub ml.(stack_pastend) ml.(stack_start)) / bytes_per_word in
-      if Z.ltb num_stackwords stack_words_needed then None (* not enough stack *) else Some (insts, positions)
-    | None => None
-    end.
 
   (* This lemma translates "sim", which depends on the large definition "related", into something
      more understandable and usable. *)
@@ -1167,135 +629,28 @@ case TODO.
           machine_ok p_functions f_entry_rel_pos ml.(stack_start) ml.(stack_pastend) instrs
                      p_call (word.add p_call (word.of_Z 4)) mH' Rdata Rexec final).
   Proof.
-    intros. unfold compile in *. simp. eapply Z.ltb_ge in E0.
-    eapply runsTo_weaken.
-    - pose proof sim' as P. eapply simulation_alt in P.
-      unfold simulation_without_weakening, SrcState, srcExec in P.
-      let x := open_constr:((_, _, false, _, _, _, _):
-        Semantics.env * Syntax.cmd.cmd * bool * Semantics.trace * Semantics.mem * Semantics.locals * MetricLog)
-      in specialize P with (s1 := x).
-      let x := open_constr:((_, _): Semantics.env * Syntax.cmd.cmd)
-      in specialize P with (f1 := x).
-      specialize P with (P1 := fun '(e', c', done', t', m', l', mc') =>
-                 e' = functions /\ c' = Syntax.cmd.call [] f_entry_name [] /\ done' = true /\ postH t' m').
-      let x := open_constr:({| p_sp := _ |}) in specialize (P x initial).
-      simpl in P.
-      eapply P; clear P.
-      + repeat match goal with
-               | |- _ /\ _ => split
-               | |- exists _, _ => eexists
-               | |- _ => reflexivity
-               | |- _ => eassumption
-               end.
-      + split; [reflexivity|].
-        eapply Semantics.exec.call; try eassumption || reflexivity.
-        cbv beta. intros.
-        repeat match goal with
-               | |- _ /\ _ => split
-               | |- exists _, _ => eexists
-               | |- _ => reflexivity
-               | |- _ => eassumption
-               end.
-    - cbv beta. intros. simp. eexists. split; [eassumption|].
-      match goal with
-      | H: ?P |- ?Q => let hP := head_of_app P in let hQ := head_of_app Q in constr_eq hP hQ;
-                       replace Q with P; [exact H|f_equal]
-      end.
-      + blia.
-      + rename H0p0p3p5 into A. clear -A h.
-        (* TODO how to automate this one? *)
-        apply (f_equal word.of_Z) in A. rewrite ?@word.of_Z_unsigned in A. 2,3: typeclasses eauto.
-        apply (f_equal (word.sub (stack_pastend ml))) in A.
-        ring_simplify in A.
-        symmetry in A.
-        exact A.
-      + congruence.
-    Unshelve. all: try exact map.empty.
-  Qed.
-
-  (* Old proof: *)
-  Goal forall
-      (ml: MemoryLayout)
-      (mlOk: MemoryLayoutOk ml)
-      (f_entry_name : string) (fbody: Syntax.cmd.cmd) (f_entry_rel_pos: Z)
-      (p_call p_functions: word)
-      (Rdata Rexec : mem -> Prop)
-      (functions: source_env)
-      (instrs: list Instruction)
-      (pos_map: funname_env Z)
-      (mH: mem) (mc: MetricLog)
-      (postH: Semantics.trace -> Semantics.mem -> Prop)
-      (initial: MetricRiscvMachine),
-      ExprImp.valid_funs functions ->
-      compile ml functions = Some (instrs, pos_map) ->
-      map.get functions f_entry_name = Some (nil, nil, fbody) ->
-      map.get pos_map f_entry_name = Some f_entry_rel_pos ->
-      Semantics.exec functions fbody initial.(getLog) mH map.empty mc (fun t' m' l' mc' => postH t' m') ->
-      machine_ok p_functions f_entry_rel_pos ml.(stack_start) ml.(stack_pastend) instrs
-                 p_call p_call mH Rdata Rexec initial ->
-      runsTo initial (fun final => exists mH',
-          postH final.(getLog) mH' /\
-          machine_ok p_functions f_entry_rel_pos ml.(stack_start) ml.(stack_pastend) instrs
-                     p_call (word.add p_call (word.of_Z 4)) mH' Rdata Rexec final).
-  Proof.
     intros.
     match goal with
     | H: map.get pos_map _ = Some _ |- _ => rename H into GetPos
     end.
-    unfold compile, composed_compile, composePhases, flattenPhase, renamePhase, spillingPhase in *. simp.
-
-    match goal with
-    | H: flatten_functions _ = _ |- _ => rename H into FlattenEq
-    end.
-    unfold flatten_functions in FlattenEq.
-    match goal with
-    | H: _ |- _ => unshelve epose proof (map.map_all_values_fw _ _ _ _ FlattenEq _ _ H)
-    end.
-    simp.
-    match goal with
-    | H: rename_functions _ = _ |- _ => rename H into RenameEq
-    end.
-    unfold rename_functions in RenameEq.
-    match goal with
-    | H: _ |- _ => unshelve epose proof (map.map_all_values_fw _ _ _ _ RenameEq _ _ H)
-    end.
-    simp.
-    match goal with
-    | H: flatten_function _ = _ |- _ => rename H into FF
-    end.
-    unfold flatten_function in FF. simp.
-
+    unfold compile, composePhases, renamePhase, flattenPhase in *. simp.
     eapply runsTo_weaken.
-    - pose proof sim as P. eapply simulation_alt in P.
-      unfold simulation_without_weakening, SrcState, srcExec in P.
-      let x := open_constr:((_, _, _, _, _, _, _):
-        Semantics.env * Syntax.cmd.cmd * bool * Semantics.trace * Semantics.mem * Semantics.locals * MetricLog)
-      in specialize P with (s1 := x).
-      let x := open_constr:((_, _): Semantics.env * Syntax.cmd.cmd)
-      in specialize P with (f1 := x).
-      specialize P with (P1 := fun '(e', c', done', t', m', l', mc') =>
-                                 e' = functions /\ c' = fbody /\ done' = true /\ postH t' m').
+    - pose proof sim as P. unfold simulation, ExprImp.SimState, ExprImp.SimExec in P.
+      specialize (P ml f_entry_rel_pos f_entry_name p_call p_functions Rdata Rexec).
+      specialize P with (e1 := functions) (s1 := (initial.(getLog), mH, map.empty, mc)).
+      specialize P with (post1 := fun '(t', m', l', mc') => postH t' m').
       simpl in P.
-      eapply P; clear P. 2: {
-        split; [reflexivity|]. eapply ExprImp.weaken_exec. 1: eassumption.
-        cbv beta. eauto.
+      eapply P; clear P; cycle -1. {
+        econstructor.
+        + eassumption.
+        + reflexivity.
+        + unfold map.of_list_zip, map.putmany_of_list_zip. reflexivity.
+        + eassumption.
+        + intros. exists nil. split; [reflexivity|].
+          exists map.empty. split; [reflexivity|].
+          eassumption.
       }
-      unfold related, flattening_related, renaming_related, spilling_related, flat_related_to_riscv,
-             compose_related.
-      eexists (_, _), (_, _, _, _, _, _, _).
-      all: admit.
-      (*
-      ssplit; try reflexivity; eauto.
-      { eexists.
-        match goal with
-        | |- ?x = (?evar1, ?evar2) => transitivity (fst x, snd x)
-        end.
-        2: reflexivity.
-        match goal with
-        | |- ?x = (_, _) => destruct x; reflexivity
-        end. }
-      eexists (_, _), (_, _, _, _, _, _, _).
-      ssplit; try reflexivity; eauto.
+      { eassumption. }
       { unfold envs_related.
         intros f [ [argnames resnames] body1 ] G.
         unfold rename_functions in *.
@@ -1303,14 +658,89 @@ case TODO.
         5: exact G. 4: eassumption.
         - eapply String.eqb_spec.
         - typeclasses eauto.
-        - simpl. typeclasses eauto.
+        - typeclasses eauto.
       }
+      { reflexivity. }
+      { unfold machine_ok in *. simp. solve_divisibleBy4. }
+      { unfold riscvPhase, machine_ok in *. simp.
+        eapply program_mod_4_0. 2: ecancel_assumption.
+        destruct (map.map_all_values_fw _ _ _ _ E _ _ H1) as [ [ [args' rets'] fbody' ] [ F G ] ].
+        unfold flatten_function in F. simp.
+        epose proof (map.map_all_values_fw _ _ _ _ E0 _ _ G) as [ [ [args' rets'] fbody' ] [ F G' ] ].
+        unfold rename_fun in F. simp.
+        eapply compile_funs_nonnil; eassumption.
+      }
+      { unfold riscvPhase in *. simp. exact GetPos. }
+      { simpl. unfold riscvPhase in *. simpl in *. simp.
+        move E1 at bottom.
+        eapply fits_stack_seq. 1: eapply fits_stack_skip. 1: reflexivity. {
+          eapply Z.div_pos.
+          - eapply proj1. eapply word.unsigned_range.
+          - clear. unfold bytes_per_word, Memory.bytes_per.
+            destruct width_cases as [E | E]; rewrite E; reflexivity.
+        }
+        destruct (map.map_all_values_fw _ _ _ _ E _ _ H1) as [ [ [args' rets'] fbody' ] [ F G ] ].
+        unfold flatten_function in F. simp.
+        epose proof (map.map_all_values_fw _ _ _ _ E0 _ _ G) as [ [ [args' rets'] fbody' ] [ F G' ] ].
+        unfold rename_fun in F. simp.
+        apply_in_hyps rename_binds_preserves_length.
+        destruct rets'; [|discriminate].
+        destruct args'; [|discriminate].
+        repeat match goal with
+               | H: _ |- _ => autoforward with typeclass_instances in H
+               end.
+        econstructor. 1: reflexivity. 1: eassumption.
+        eapply fits_stack_monotone.
+        1: eapply stack_usage_correct; eassumption. 1: reflexivity. blia. }
+      { unfold good_e_impl.
+        intros.
+        simpl in *.
+        match goal with
+        | H: rename_functions _ = _ |- _ => rename H into RenameEq
+        end.
+        unfold rename_functions in RenameEq.
+        match goal with
+        | H: _ |- _ => unshelve epose proof (map.map_all_values_bw _ _ _ _ RenameEq _ _ H)
+        end.
+        simp. destruct v1 as [ [argnames' retnames'] body' ].
+        match goal with
+        | H: flatten_functions _ _ = _ |- _ => rename H into FlattenEq
+        end.
+        unfold flatten_functions in FlattenEq.
+        match goal with
+        | H: _ |- _ => unshelve epose proof (map.map_all_values_bw _ _ _ _ FlattenEq _ _ H) as P
+        end.
+        unfold flatten_function in P.
+        simp.
+        match goal with
+        | H: ExprImp.valid_funs _ |- _ => rename H into V
+        end.
+        unfold ExprImp.valid_funs in V.
+        specialize V with (1 := Pp1).
+        unfold ExprImp.valid_fun in V.
+        destruct V.
+        ssplit.
+        - eapply rename_fun_valid; try eassumption.
+          unfold ExprImp2FlatImp in *.
+          simp.
+          repeat match goal with
+                 | H: @eq bool _ _ |- _ => autoforward with typeclass_instances in H
+                 end.
+          assumption.
+        - unfold FlatToRiscvDef.build_fun_pos_env, FlatToRiscvDef.build_fun_pos_env.
+          pose proof (get_compile_funs_pos r0) as P.
+          destruct (FlatToRiscvDef.compile_funs map.empty r0) as [ insts posmap ] eqn: F.
+          eapply P.
+          eassumption.
+      }
+      unfold related, compose_relation.
+      unfold FlatToRiscvSimulation.related, FlattenExprSimulation.related, RegRename.related.
+      refine (ex_intro _ (_, _, _, _) _).
+      ssplit; try reflexivity.
       refine (ex_intro _ (_, _, _, _) _).
       ssplit; try reflexivity.
       { intros. ssplit; reflexivity. }
-      { unfold machine_ok in *. simp.
-        (* PARAMRECORDS *) simpl.
-        solve_word_eq word_ok. }
+      { unfold machine_ok in *. simp. simpl_param_projections. solve_word_eq word_ok. }
       unfold goodMachine. simpl. ssplit.
       { simpl. unfold map.extends. intros k v Emp. rewrite map.get_empty in Emp. discriminate. }
       { simpl. unfold map.extends. intros k v Emp. rewrite map.get_empty in Emp. discriminate. }
@@ -1347,7 +777,6 @@ case TODO.
           symmetry in P.
           simpl in P|-*. unfold program in P.
           seprewrite P. clear P.
-          assert (word.ok FlatImp.word) by exact word_ok.
           rewrite <- Z_div_exact_2; cycle 1. {
             unfold bytes_per_word. clear -h.
             destruct width_cases as [E | E]; rewrite E; reflexivity.
@@ -1359,13 +788,13 @@ case TODO.
             apply stack_length_divisible.
             assumption.
           }
-          wcancel_assumption.
-          rewrite word.of_Z_unsigned.
-          cancel_seps_at_indices O O. {
-            (* PARAMRECORDS *) simpl.
-            sepclause_eq word_ok.
-          }
-          cbn [seps]. reflexivity.
+          ParamRecords.simpl_param_projections.
+          use_sep_assumption.
+          unfold ptsto_bytes.
+          wseplog_pre.
+          simpl_addrs.
+          rewrite !word.of_Z_unsigned.
+          wcancel.
         }
         match goal with
         | E: Z.of_nat _ = word.unsigned (word.sub _ _) |- _ => simpl in E|-*; rewrite <- E
@@ -1374,8 +803,7 @@ case TODO.
         apply Hlength_stack_trash_words. }
       { reflexivity. }
       { unfold machine_ok in *. simp. assumption. }
-      *)
-    - intros. unfold compile_inv, related, compose_related in *.
+    - intros. unfold compile_inv, related, compose_relation in *.
       match goal with
       | H: context[machine_ok] |- _ =>
         unfold machine_ok in H;
@@ -1392,15 +820,11 @@ case TODO.
       repeat match goal with
              | H: context[Semantics.exec] |- _ => clear H
              end.
-      unfold flattening_related, renaming_related, spilling_related, flat_related_to_riscv in *.
       unfold FlatToRiscvSimulation.related, FlattenExprSimulation.related, RegRename.related, goodMachine in *.
-      admit.
-      (*
       simp.
       eexists. split. 1: eassumption.
       unfold machine_ok. ssplit; try assumption.
-      + assert (map.ok mem). { exact mem_ok. } (* PARAMRECORDS *)
-        cbv [rem_stackwords rem_framewords ghostConsts] in H2p0p1p8p0.
+      + cbv [rem_stackwords rem_framewords ghostConsts] in H2p0p1p8p0.
         cbv [mem_available].
         repeat rewrite ?(iff1ToEq (sep_ex1_r _ _)), ?(iff1ToEq (sep_ex1_l _ _)).
         exists (List.flat_map (fun x => HList.tuple.to_list (LittleEndian.split (Z.to_nat bytes_per_word) (word.unsigned x))) stack_trash).
@@ -1446,7 +870,6 @@ case TODO.
         simpl.
         unfold ptsto_bytes, ptsto_instr, truncated_scalar, littleendian, ptsto_bytes.ptsto_bytes.
         simpl.
-        assert (map.ok mem). { exact mem_ok. } (* PARAMRECORDS *)
         wwcancel.
         epose proof (functions_to_program ml _ r0 instrs) as P.
         cbn [seps].
@@ -1469,7 +892,6 @@ case TODO.
         simpl.
         wwcancel.
       + destr_RiscvMachine final. subst. solve_divisibleBy4.
-      *)
     Unshelve.
     all: try exact (bedrock2.MetricLogging.mkMetricLog 0 0 0 0).
     all: try (simpl; typeclasses eauto).
@@ -1477,7 +899,7 @@ case TODO.
     all: try exact nil.
     all: try exact map.empty.
     all: try exact mem_ok.
-  Abort.
+  Qed.
 
   Definition instrencode(p: list Instruction): list byte :=
     List.flat_map (fun inst => HList.tuple.to_list (LittleEndian.split 4 (encode inst))) p.
